Add uint32 support

src/dafny_go/encoding/encoding_test.go
@@ -19,6 +19,18 @@ func TestEncodeOf0(t *testing.T) {
 		"encoding of zero is not 8 zeros")
 }
 
+func TestEncodeOf0_32(t *testing.T) {
+	bs := bytes.NewBytes(4)
+	for i := 0; i < 4; i++ {
+		bs.Data[i] = 1
+	}
+
+	UInt32Put(0, 0, bs)
+
+	assert.Equal(t, []byte{0, 0, 0, 0}, bs.Data[:4],
+		"encoding of zero (32-bit) is not 4 zeros")
+}
+
 func TestEncodeDecodeAt0(t *testing.T) {
 	assert := assert.New(t)
 	for _, x := range []uint64{
@@ -42,4 +54,29 @@ func TestEncodeDecodeOffset(t *testing.T) {
 	bs = bytes.NewBytes(4 + 8)
 	UInt64Put(x, 4, bs)
 	assert.Equal(x, UInt64Get(bs, 4))
+}
+
+func TestEncodeDecodeAt0_32(t *testing.T) {
+	assert := assert.New(t)
+	for _, x := range []uint32{
+		0, 1,
+		0xFFFF_FFFF,
+		0x0102_0304,
+	} {
+		bs := bytes.NewBytes(8)
+		UInt32Put(x, 0, bs)
+		assert.Equal(x, UInt32Get(bs, 0))
+	}
+}
+
+func TestEncodeDecodeOffset_32(t *testing.T) {
+	assert := assert.New(t)
+	var x uint32 = 0x0102_0304
+	bs := bytes.NewBytes(16)
+	UInt32Put(x, 4, bs)
+	assert.Equal(x, UInt32Get(bs, 4))
+
+	bs = bytes.NewBytes(4 + 8)
+	UInt32Put(x, 4, bs)
+	assert.Equal(x, UInt32Get(bs, 4))
 }
