src/Dafny/machine/int_encoding.s.dfy
@@ -11,24 +11,49 @@ module {:extern "encoding", "github.com/mit-pdos/dafny-jrnl/src/dafny_go/encodin
     import opened Machine
     import opened ByteSlice
 
+    const u64_bytes: nat := 8
+    const u32_bytes: nat := 4
+
     function method {:axiom} le_enc64(x: uint64): (bs:seq<byte>)
-        ensures |bs| == 8
+        ensures |bs| == u64_bytes
     function method {:axiom} le_dec64(bs: seq<byte>): uint64
-        requires |bs| == 8
+        requires |bs| == u64_bytes
     lemma {:axiom} lemma_le_enc_dec64(x: uint64)
         ensures le_dec64(le_enc64(x)) == x
     lemma {:axiom} lemma_enc_0()
         ensures le_enc64(0) == [0,0,0,0,0,0,0,0]
 
+    function method {:axiom} le_enc32(x: uint32): (bs:seq<byte>)
+        ensures |bs| == u32_bytes
+    function method {:axiom} le_dec32(bs: seq<byte>): uint32
+        requires |bs| == u32_bytes
+    lemma {:axiom} lemma_le_enc_dec32(x: uint32)
+        ensures le_dec32(le_enc32(x)) == x
+    lemma {:axiom} lemma_enc_32_0()
+        ensures le_enc32(0) == [0,0,0,0]
+
     method {:extern} UInt64Put(x: uint64, off: uint64, bytes: Bytes)
     modifies bytes
     requires bytes.Valid() ensures bytes.Valid()
-    requires off as nat + 8 <= |bytes.data|
-    ensures bytes.data == old(bytes.data[..off as nat] + le_enc64(x) + bytes.data[off as nat+8..])
+    requires off as nat + u64_bytes <= |bytes.data|
+    ensures bytes.data == old(bytes.data[..off as nat] + le_enc64(x) + bytes.data[off as nat+u64_bytes..])
 
     method {:extern} UInt64Get(bytes: Bytes, off: uint64)
     returns (x:uint64)
     requires bytes.Valid()
-    requires off as nat + 8 <= |bytes.data|
-    ensures x == le_dec64(bytes.data[off as nat..off as nat+8])
+    requires off as nat + u64_bytes <= |bytes.data|
+    ensures x == le_dec64(bytes.data[off as nat..off as nat+u64_bytes])
+
+    method {:extern} UInt32Put(x: uint32, off: uint32, bytes: Bytes)
+    modifies bytes
+    requires bytes.Valid() ensures bytes.Valid()
+    requires off as nat + u32_bytes <= |bytes.data|
+    ensures bytes.data == old(bytes.data[..off as nat] + le_enc32(x) + bytes.data[off as nat+u32_bytes..])
+
+    method {:extern} UInt32Get(bytes: Bytes, off: uint32)
+    returns (x:uint32)
+    requires bytes.Valid()
+    requires off as nat + u32_bytes <= |bytes.data|
+    ensures x == le_dec32(bytes.data[off as nat..off as nat+u32_bytes])
+
 }
